src/Compilers/CommonSubexpressionEliminationInterp.v
@@ -40,7 +40,8 @@ Section symbolic.
           (symbolize_op : forall s d, op s d -> op_code)
           (denote_op : forall s d, op_code -> option (op s d)).
   Local Notation symbolic_expr := (symbolic_expr base_type_code op_code).
-  Context (normalize_symbolic_op_arguments : op_code -> symbolic_expr -> symbolic_expr).
+  Context (normalize_symbolic_op_arguments : op_code -> symbolic_expr -> symbolic_expr)
+          (inline_symbolic_expr_in_lookup : bool).
 
   Local Notation symbolic_expr_beq := (@symbolic_expr_beq base_type_code op_code base_type_code_beq op_code_beq).
   Local Notation symbolic_expr_lb := (@internal_symbolic_expr_dec_lb base_type_code op_code base_type_code_beq op_code_beq base_type_code_lb op_code_lb).
@@ -57,9 +58,9 @@ Section symbolic.
 
   Local Notation symbolicify_smart_var := (@symbolicify_smart_var base_type_code op_code).
   Local Notation symbolize_exprf := (@symbolize_exprf base_type_code op_code op symbolize_op).
-  Local Notation csef := (@csef base_type_code op_code base_type_code_beq op_code_beq base_type_code_bl op symbolize_op normalize_symbolic_op_arguments).
-  Local Notation cse := (@cse base_type_code op_code base_type_code_beq op_code_beq base_type_code_bl op symbolize_op normalize_symbolic_op_arguments).
-  Local Notation CSE := (@CSE base_type_code op_code base_type_code_beq op_code_beq base_type_code_bl op symbolize_op normalize_symbolic_op_arguments).
+  Local Notation csef := (@csef base_type_code op_code base_type_code_beq op_code_beq base_type_code_bl op symbolize_op normalize_symbolic_op_arguments inline_symbolic_expr_in_lookup).
+  Local Notation cse := (@cse base_type_code op_code base_type_code_beq op_code_beq base_type_code_bl op symbolize_op normalize_symbolic_op_arguments inline_symbolic_expr_in_lookup).
+  Local Notation CSE := (@CSE base_type_code op_code base_type_code_beq op_code_beq base_type_code_bl op symbolize_op normalize_symbolic_op_arguments inline_symbolic_expr_in_lookup).
   Local Notation SymbolicExprContext := (@SymbolicExprContext base_type_code op_code base_type_code_beq op_code_beq base_type_code_bl).
   Local Notation SymbolicExprContextOk := (@SymbolicExprContextOk base_type_code op_code base_type_code_beq op_code_beq base_type_code_bl base_type_code_lb op_code_bl op_code_lb).
   Local Notation prepend_prefix := (@prepend_prefix base_type_code op).
