src/Compilers/Z/CommonSubexpressionEliminationWf.v
@@ -5,7 +5,7 @@ Require Import Crypto.Compilers.Z.Syntax.
 Require Import Crypto.Compilers.CommonSubexpressionEliminationWf.
 Require Import Crypto.Compilers.Z.CommonSubexpressionElimination.
 
-Lemma Wf_CSE_gen t (e : Expr _ _ t)
+Lemma Wf_CSE_gen inline_symbolic_expr_in_lookup t (e : Expr _ _ t)
       prefix
       (Hlen : forall var1 var2, length (prefix var1) = length (prefix var2))
       (Hprefix : forall var1 var2 n t1 t2 e1 e2,
@@ -13,14 +13,14 @@ Lemma Wf_CSE_gen t (e : Expr _ _ t)
           -> List.nth_error (prefix var2) n = Some (existT _ t2 e2)
           -> exists pf : t1 = t2, wff nil (eq_rect _ (@exprf _ _ _) e1 _ pf) e2)
       (Hwf : Wf e)
-  : Wf (@CSE_gen t e prefix).
+  : Wf (@CSE_gen inline_symbolic_expr_in_lookup t e prefix).
 Proof.
   apply Wf_CSE; auto using internal_base_type_dec_bl, internal_base_type_dec_lb, internal_symbolic_op_dec_bl, internal_symbolic_op_dec_lb.
 Qed.
 
-Lemma Wf_CSE t (e : Expr _ _ t)
+Lemma Wf_CSE inline_symbolic_expr_in_lookup t (e : Expr _ _ t)
       (Hwf : Wf e)
-  : Wf (@CSE t e).
+  : Wf (@CSE inline_symbolic_expr_in_lookup t e).
 Proof.
   apply Wf_CSE_gen; simpl; auto.
   { destruct n; simpl; try congruence. }
